introduced a timestamp type (not neccessarily for hiding, but for better readability of function types)

src/core/DY.Core.Trace.Type.fst
@@ -64,12 +64,16 @@ let rec length tr =
   | Nil -> 0
   | Snoc init last -> length init + 1
 
+/// a type macro for timestamps (indices on the trace)
+
+type timestamp = nat
+
 (*** Prefix and trace extension ***)
 
 /// Compute the prefix of a trace.
 
 [@@ "opaque_to_smt"]
-val prefix: tr:trace -> i:nat{i <= length tr} -> trace
+val prefix: tr:trace -> i:timestamp{i <= length tr} -> trace
 let rec prefix tr i =
   if length tr = i then
     tr
@@ -122,7 +126,7 @@ let rec grows_transitive tr1 tr2 tr3 =
 /// The prefix function outputs traces of the correct length.
 
 val length_prefix:
-  tr:trace -> i:nat{i <= length tr} ->
+  tr:trace -> i:timestamp{i <= length tr} ->
   Lemma
   (ensures length (prefix tr i) == i)
   [SMTPat (length (prefix tr i))]
@@ -147,7 +151,7 @@ let length_grows tr1 tr2 =
 /// The prefix function outputs traces that are prefixes of the input.
 
 val prefix_grows:
-  tr:trace -> i:nat{i <= length tr} ->
+  tr:trace -> i:timestamp{i <= length tr} ->
   Lemma
   (ensures (prefix tr i) <$ tr)
   //TODO: is this SMTPat dangerous? Should we restrict it to the "safe" on below?
@@ -158,7 +162,7 @@ let prefix_grows tr i =
   norm_spec [zeta; delta_only [`%prefix]] (prefix)
 
 val prefix_prefix_grows:
-  tr1:trace -> tr2:trace -> i1:nat -> i2:nat ->
+  tr1:trace -> tr2:trace -> i1:timestamp -> i2:timestamp ->
   Lemma
   (requires
     tr1 <$ tr2 /\
@@ -186,7 +190,7 @@ let rec prefix_prefix_grows tr1 tr2 i1 i2 =
   )
 
 val prefix_prefix_eq:
-  tr1:trace -> tr2:trace -> i:nat ->
+  tr1:trace -> tr2:trace -> i:timestamp ->
   Lemma
   (requires
     tr1 <$ tr2 /\
@@ -209,7 +213,7 @@ let rec prefix_prefix_eq tr1 tr2 i =
 
 /// Retrieve the event at some timestamp in the trace.
 
-val get_event_at: tr:trace -> i:nat{i < length tr} -> trace_event
+val get_event_at: tr:trace -> i:timestamp{i < length tr} -> trace_event
 let rec get_event_at tr i =
   if i+1 = length tr then
     let Snoc _ last = tr in
@@ -221,7 +225,7 @@ let rec get_event_at tr i =
 
 /// Has some particular event been triggered at a some particular timestamp in the trace?
 
-val event_at: trace -> nat -> trace_event -> prop
+val event_at: trace -> timestamp -> trace_event -> prop
 let event_at tr i e =
   if i >= length tr then
     False
@@ -238,7 +242,7 @@ let event_exists tr e =
 
 val event_at_grows:
   tr1:trace -> tr2:trace ->
-  i:nat -> e:trace_event ->
+  i:timestamp -> e:trace_event ->
   Lemma
   (requires event_at tr1 i e /\ tr1 <$ tr2)
   (ensures event_at tr2 i e)
@@ -275,7 +279,7 @@ let was_corrupt tr prin sess_id =
 
 /// Has a (custom, protocol-specific) event been triggered at some timestamp?
 
-val event_triggered_at: trace -> nat -> principal -> string -> bytes -> prop
+val event_triggered_at: trace -> timestamp -> principal -> string -> bytes -> prop
 let event_triggered_at tr i prin tag content =
   event_at tr i (Event prin tag content)
 
@@ -298,7 +302,7 @@ let event_triggered_grows tr1 tr2 prin tag content = ()
 
 /// Has a random bytestring been generated at some timestamp?
 
-val rand_generated_at: trace -> nat -> bytes -> prop
+val rand_generated_at: trace -> timestamp -> bytes -> prop
 let rand_generated_at tr i b =
   match b with
   | Rand usg lab len time ->
